Veltman semantics adhoc fix

Foundation/InterpretabilityLogic/Veltman/Logic/CL.lean
@@ -7,11 +7,13 @@ open Veltman
 
 namespace Veltman
 
-protected abbrev FrameClass.CL : FrameClass := Set.univ
+protected abbrev FrameClass.CL : FrameClass := { F | F.IsCL }
 
 abbrev trivialFrame : Veltman.Frame where
   toKripkeFrame := Modal.Kripke.blackpoint
   S _ _ _ := True
+
+instance : Veltman.trivialFrame.IsCL where
   S_refl _ := ⟨by tauto⟩
   S_trans _ := ⟨by tauto⟩
 
@@ -20,16 +22,20 @@ end Veltman
 
 namespace CL
 
-instance Veltman.sound : Sound InterpretabilityLogic.CL FrameClass.CL := instSound_of_validates_axioms $ by
-  constructor;
-  intro φ hφ;
-  have := (show CL.axioms ∪ ∅ = CL.axioms by simp) ▸ validates_CL_axioms_union (Ax := ∅) (C := FrameClass.CL) ⟨by tauto⟩;
-  apply this.models;
-  assumption;
+instance Veltman.sound : Sound InterpretabilityLogic.CL FrameClass.CL := by
+  apply instSound_of_validates_axioms;
+  . intro F hF;
+    replace hF := Set.mem_setOf_eq.mp hF;
+    infer_instance;
+  . constructor;
+    intro φ hφ F hF;
+    replace hF := Set.mem_setOf_eq.mp hF;
+    rcases hφ with (rfl | rfl | rfl | rfl) <;> simp;
 
 instance : Entailment.Consistent InterpretabilityLogic.CL := consistent_of_sound_frameclass FrameClass.CL $ by
   use Veltman.trivialFrame;
-  simp;
+  apply Set.mem_setOf_eq.mpr;
+  infer_instance;
 
 end CL
 
