Foundation/InterpretabilityLogic/Veltman/Hilbert.lean
@@ -1,4 +1,4 @@
-import Foundation.InterpretabilityLogic.Hilbert.Basic
+import Foundation.InterpretabilityLogic.Hilbert.Basic.Basic
 import Foundation.InterpretabilityLogic.Veltman.Basic
 
 namespace LO.InterpretabilityLogic
@@ -11,9 +11,9 @@ namespace Veltman
 variable {Ax Ax₁ Ax₂ : Axiom ℕ} {φ : Formula ℕ}
 variable {F : Frame} {C : FrameClass}
 
-lemma soundness_of_validates_axioms (hV : C ⊧* Ax) : Hilbert Ax ⊢ φ → C ⊧ φ := by
+lemma soundness_of_validates_axioms (hGL : ∀ F ∈ C, F.IsInfiniteGL) (hV : C ⊧* Ax) : Hilbert.Basic Ax ⊢ φ → C ⊧ φ := by
   intro hφ F hF;
-  induction hφ using Hilbert.rec! with
+  induction hφ using Hilbert.Basic.rec! with
   | @axm φ s h =>
     apply ValidOnFrame.subst;
     apply hV.models;
@@ -24,15 +24,17 @@ lemma soundness_of_validates_axioms (hV : C ⊧* Ax) : Hilbert Ax ⊢ φ → C �
   | imply₁ => exact ValidOnFrame.imply₁;
   | imply₂ => exact ValidOnFrame.imply₂;
   | ec => exact ValidOnFrame.elimContra;
+  | axiomK => exact ValidOnFrame.axiomK;
+  | axiomL => have := hGL F hF; exact ValidOnFrame.axiomL;
 
-instance instSound_of_validates_axioms (hV : C ⊧* Ax) : Sound (Hilbert Ax) C := ⟨fun {_} =>
-  soundness_of_validates_axioms hV
+instance instSound_of_validates_axioms (hGL : ∀ F ∈ C, F.IsInfiniteGL) (hV : C ⊧* Ax) : Sound (Hilbert.Basic Ax) C := ⟨fun {_} =>
+  soundness_of_validates_axioms hGL hV
 ⟩
 
 lemma consistent_of_sound_frameclass
   (C : Veltman.FrameClass) (C_nonempty: C.Nonempty)
-  [sound : Sound (Hilbert Ax) C]
-  : Entailment.Consistent (Hilbert Ax) := by
+  [sound : Sound (Hilbert.Basic Ax) C]
+  : Entailment.Consistent (Hilbert.Basic Ax) := by
   apply Entailment.Consistent.of_unprovable (φ := ⊥);
   apply not_imp_not.mpr sound.sound;
   apply Semantics.set_models_iff.not.mpr;
@@ -44,9 +46,9 @@ lemma consistent_of_sound_frameclass
   . simp;
 
 
-lemma soundness_of_frame_validates_axioms (hV : F ⊧* Ax) : (Hilbert Ax) ⊢ φ → F ⊧ φ := by
+lemma soundness_of_frame_validates_axioms [F.IsInfiniteGL] (hV : F ⊧* Ax) : (Hilbert.Basic Ax) ⊢ φ → F ⊧ φ := by
   intro hφ;
-  induction hφ using Hilbert.rec! with
+  induction hφ using Hilbert.Basic.rec! with
   | axm s h =>
     apply ValidOnFrame.subst;
     apply hV.models;
@@ -56,20 +58,22 @@ lemma soundness_of_frame_validates_axioms (hV : F ⊧* Ax) : (Hilbert Ax) ⊢ φ
   | imply₁ => exact ValidOnFrame.imply₁;
   | imply₂ => exact ValidOnFrame.imply₂;
   | ec => exact ValidOnFrame.elimContra;
+  | axiomK => exact ValidOnFrame.axiomK;
+  | axiomL => exact ValidOnFrame.axiomL;
 
-instance instSound_of_frame_validates_axioms (hV : F ⊧* Ax) : Sound (Hilbert Ax) F := ⟨fun {_} =>
+instance instSound_of_frame_validates_axioms [F.IsInfiniteGL] (hV : F ⊧* Ax) : Sound (Hilbert.Basic Ax) F := ⟨fun {_} =>
   soundness_of_frame_validates_axioms hV
 ⟩
 
-lemma consistent_of_sound_frames (F : Veltman.Frame) [sound : Sound (Hilbert Ax) F] : Entailment.Consistent (Hilbert Ax) := by
+lemma consistent_of_sound_frames (F : Veltman.Frame) [sound : Sound (Hilbert.Basic Ax) F] : Entailment.Consistent (Hilbert.Basic Ax) := by
   apply Entailment.Consistent.of_unprovable (φ := ⊥);
   apply not_imp_not.mpr sound.sound;
   exact Veltman.ValidOnFrame.bot_def;
 
 lemma weakerThan_of_subset_frameClass
   (C₁ C₂ : FrameClass) (hC : C₂ ⊆ C₁)
-  [Sound (Hilbert Ax₁) C₁] [Complete (Hilbert Ax₂) C₂]
-  : (Hilbert Ax₁) ⪯ (Hilbert Ax₂) := by
+  [Sound (Hilbert.Basic Ax₁) C₁] [Complete (Hilbert.Basic Ax₂) C₂]
+  : (Hilbert.Basic Ax₁) ⪯ (Hilbert.Basic Ax₂) := by
   apply Entailment.weakerThan_iff.mpr;
   intro φ hφ;
   apply Complete.complete (𝓜 := C₂);
@@ -77,6 +81,7 @@ lemma weakerThan_of_subset_frameClass
   apply Sound.sound (𝓜 := C₁) hφ;
   apply hC hF;
 
+/-
 lemma validates_CL_axioms_union (hV : C ⊧* Ax) : C ⊧* CL.axioms ∪ Ax := by
   constructor;
   rintro φ ((rfl | rfl | rfl | rfl | rfl | rfl) | hφ);
@@ -88,6 +93,7 @@ lemma validates_CL_axioms_union (hV : C ⊧* Ax) : C ⊧* CL.axioms ∪ Ax := by
   . intro _ _; apply ValidOnFrame.axiomJ4;
   . apply hV.models;
     assumption;
+-/
 
 end Veltman
 
